More decidable typechecking, working on decrease fun and pred
Change definition in typing to decidable, but will change back
Through fun case, some easier, most of way through match case

proofs/core/Typechecker.v
@@ -714,6 +714,7 @@ Qed.
 
 Section ContextCheck.
 
+Variable sigma: sig.
 Variable gamma: context.
 
 (*Here, we show that the context checks (some of them for now)
@@ -843,6 +844,609 @@ Definition check_valid_matches_tm_spec t :=
   fst (check_valid_matches_spec t Ftrue).
 Definition check_valid_matches_fmla_spec f := 
   snd (check_valid_matches_spec tm_d f).
+
+(*Well-typed terms*)
+Definition check_well_typed_tm (t: term) (ty: vty) : bool :=
+  (typecheck_term sigma t == Some ty) &&
+  check_valid_matches_tm t.
+
+Definition check_well_typed_fmla (f: formula) : bool :=
+  (typecheck_formula sigma f) &&
+  check_valid_matches_fmla f.
+
+Lemma check_well_typed_tm_spec (t: term) (ty: vty):
+  reflect (well_typed_term sigma gamma t ty) (check_well_typed_tm t ty).
+Proof.
+  apply andPP.
+  apply typecheck_term_correct.
+  apply check_valid_matches_tm_spec.
+Qed.
+
+Lemma check_well_typed_fmla_spec (f: formula):
+  reflect (well_typed_formula sigma gamma f) (check_well_typed_fmla f).
+Proof.
+  apply andPP.
+  apply typecheck_formula_correct.
+  apply check_valid_matches_fmla_spec.
+Qed.
+
+(*TODO: [adt_valid_type], inhabited types, strict positivity
+  for types (TODO: add uniformity)*)
+
+(*Checks for recursive functions*)
+
+(*TODO: duplicates [check_sublist] in Syntax, but we don't use
+  ssreflect there*)
+
+Definition sublistb {A: eqType} (l1 l2: seq A) : bool :=
+  (all (fun x => x \in l2) l1).
+
+Lemma sublistbP {A: eqType} (l1 l2: seq A):
+  reflect (sublist l1 l2) (sublistb l1 l2).
+Proof.
+  rewrite /sublist/sublistb.
+  eapply equivP.
+  2: apply Forall_forall.
+  apply all_Forall. move=> x Hinx.
+  apply inP.
+Qed.
+
+(*TODO: move, maybe use instead of nodupb*)
+Lemma uniqP {A: eqType} (l: list A):
+  reflect (NoDup l) (uniq l).
+Proof.
+  elim: l => [//= | h t /= IH].
+  - reflT.
+  - eapply equivP. 2: symmetry; apply NoDup_cons_iff.
+    apply andPP=>//.
+    apply negPP. apply inP.
+Qed.
+
+Definition check_funpred_def_valid_type (fd: funpred_def) : bool :=
+  match fd with
+  | fun_def f vars t =>
+    check_well_typed_tm t (f_ret f) &&
+    sublistb (term_fv t) vars &&
+    (length vars == length (s_args f)) &&
+    uniq (map fst vars) &&
+    (map snd vars == s_args f)
+  | pred_def p vars f =>
+    check_well_typed_fmla f &&
+    sublistb (form_fv f) vars &&
+    (length vars == length (s_args p)) &&
+    uniq (map fst vars) &&
+    (map snd vars == s_args p)
+  end.
+
+Lemma check_funpred_def_valid_type_spec (fd: funpred_def):
+  reflect (funpred_def_valid_type sigma gamma fd) 
+    (check_funpred_def_valid_type fd).
+Proof.
+  rewrite /funpred_def_valid_type/check_funpred_def_valid_type.
+  case: fd => [f vars t | p vars f].
+  - rewrite -andbA -andbA -andbA. repeat (apply andPP; [|apply andPP]).
+    + apply check_well_typed_tm_spec.
+    + apply sublistbP.
+    + apply eqP.
+    + apply uniqP.
+    + apply eqP.
+  - rewrite -andbA -andbA -andbA. repeat (apply andPP; [|apply andPP]).
+    + apply check_well_typed_fmla_spec.
+    + apply sublistbP.
+    + apply eqP.
+    + apply uniqP.
+    + apply eqP.
+Qed.
+
+(*Now, we come to the core of this: finding the list of
+  indices such that the function is structurally 
+  decreasing on these indices*)
+Search find.
+
+(*Default values for fn, sn*)
+Definition sn_d : sn :=
+  (mk_sn id_sym [vs_d] 0).
+
+Definition fn_d : fn :=
+  (mk_fn id_fs sn_d tm_d).
+
+Definition pn_d : pn :=
+  (mk_pn (Build_predsym id_sym) sn_d Ftrue).
+
+
+(*First, we need a decidable version of
+  [decrease_fun] and [decrease_pred], assuming we already
+  have fs and ps*)
+(*TODO: this is likely very inefficient, and we need
+  to ensure that everything is computable*)
+Fixpoint check_decrease_fun (fs: list fn) (ps: list pn)
+  (small: list vsymbol) (hd: option vsymbol) (m: mut_adt)
+  (vs: list vty) (t: term) : bool :=
+  (*Don't use any recursive instance*)
+  (all (fun f => negb (funsym_in_tm (fn_sym f) t)) fs &&
+  all (fun p => negb (predsym_in_term (pn_sym p) t)) ps) ||
+  match t with
+  | Tfun f l ts =>
+    (*Hard case:*)
+    let idx := find (fun f' => fn_sym f' == f) fs in
+    if (idx < length fs) then
+      let f_decl := nth fn_d fs idx in
+      
+      match nth tm_d ts (sn_idx f_decl) with
+      | Tvar x => 
+        (x \in small) &&
+        (l == map vty_var (s_params f)) &&
+        all (fun t => all (fun f => negb (funsym_in_tm (fn_sym f) t)) fs) ts &&
+        all (fun t => all (fun p => negb (predsym_in_term (pn_sym p) t)) ps) ts 
+      | _ => false
+      end 
+    else 
+      (*Not recursive*)
+      all (fun t => check_decrease_fun fs ps small hd m vs t) ts
+  (*Other hard cases - pattern matches*)
+  | Tmatch (Tvar mvar) v pats =>
+    if ((hd == Some mvar) || (mvar \in small)) then 
+    (*TODO: WRONG, need to use [vty_in_m] because we check against
+      m, not everything*)
+      match (is_vty_adt gamma (snd mvar)) with
+      | Some (m', a, vs) =>
+        mut_adt_dec m m' && (*TODO: do we need mut_eqb*)
+        adt_in_mut a m &&
+        all (fun x =>
+          check_decrease_fun fs ps
+          (union vsymbol_eq_dec (vsyms_in_m m vs (pat_constr_vars m vs (fst x))) 
+          (remove_all vsymbol_eq_dec (pat_fv (fst x)) 
+          small)) (upd_option_iter hd (pat_fv (fst x))) m vs (snd x)
+          ) pats
+      | None => false
+      end
+    (*Non-smaller cases*)
+    else 
+      all (fun x =>
+        check_decrease_fun fs ps 
+        (remove_all vsymbol_eq_dec (pat_fv (fst x)) small) 
+        (upd_option_iter hd (pat_fv (fst x))) m vs (snd x)) pats
+  | Tmatch tm v pats =>
+    check_decrease_fun fs ps small hd m vs tm &&
+    all (fun x =>
+      check_decrease_fun fs ps 
+      (remove_all vsymbol_eq_dec (pat_fv (fst x)) small) 
+      (upd_option_iter hd (pat_fv (fst x))) m vs (snd x)) pats
+  | Tlet t1 v t2 =>
+    check_decrease_fun fs ps small hd m vs t1 &&
+    check_decrease_fun fs ps (remove vsymbol_eq_dec v small) (upd_option hd v) m vs t2
+  | Tif f1 t1 t2 =>
+    check_decrease_pred fs ps small hd m vs f1 &&
+    check_decrease_fun fs ps small hd m vs t1 &&
+    check_decrease_fun fs ps small hd m vs t2
+  | Teps f v =>
+    check_decrease_pred fs ps (remove vsymbol_eq_dec v small) (upd_option hd v) m vs f
+  | _ => true
+  end
+
+with check_decrease_pred (fs: list fn) (ps: list pn)
+  (small: list vsymbol) (hd: option vsymbol) (m: mut_adt)
+  (vs: list vty) (f: formula) : bool :=
+  (*Don't use any recursive instance*)
+  (all (fun f' => negb (funsym_in_fmla (fn_sym f') f)) fs &&
+  all (fun p => negb (predsym_in (pn_sym p) f)) ps) ||
+  match f with
+  | Fpred p l ts =>
+    (*Hard case:*)
+    let idx := find (fun p' => pn_sym p' == p) ps in
+    if (idx < length ps) then
+      let p_decl := nth pn_d ps idx in
+      
+      match nth tm_d ts (sn_idx p_decl) with
+      | Tvar x => 
+        (x \in small) &&
+        (l == map vty_var (s_params p)) &&
+        all (fun t => all (fun f => negb (funsym_in_tm (fn_sym f) t)) fs) ts &&
+        all (fun t => all (fun p => negb (predsym_in_term (pn_sym p) t)) ps) ts 
+      | _ => false
+      end 
+    else 
+      (*Not recursive*)
+      all (fun t => check_decrease_fun fs ps small hd m vs t) ts
+   (*Other hard cases - pattern matches*)
+   | Fmatch (Tvar mvar) v pats =>
+   ((hd == Some mvar) || (mvar \in small)) &&
+   match (is_vty_adt gamma (snd mvar)) with
+   | Some (m', a, vs) =>
+     (*mut_adt_dec m m' && (*TODO: do we need mut_eqb*)
+     adt_in_mut a m &&*)
+     all (fun x =>
+       check_decrease_pred fs ps
+       (union vsymbol_eq_dec (vsyms_in_m m vs (pat_constr_vars m vs (fst x))) 
+       (remove_all vsymbol_eq_dec (pat_fv (fst x)) 
+       small)) (upd_option_iter hd (pat_fv (fst x))) m vs (snd x)
+       ) pats
+   | None => false
+   end
+ | Fmatch tm v pats =>
+   match tm with
+   | Tvar x => (hd != Some x) && (x \notin small)
+   | _ => true
+   end &&
+   check_decrease_fun fs ps small hd m vs tm &&
+   all (fun x =>
+     check_decrease_pred fs ps 
+     (remove_all vsymbol_eq_dec (pat_fv (fst x)) small) 
+     (upd_option_iter hd (pat_fv (fst x))) m vs (snd x)) pats
+  | Fnot f =>
+    check_decrease_pred fs ps small hd m vs f 
+  | Fquant q v f =>
+    check_decrease_pred fs ps (remove vsymbol_eq_dec v small) (upd_option hd v) m vs f
+  | Feq ty t1 t2 =>
+    check_decrease_fun fs ps small hd m vs t1 &&
+    check_decrease_fun fs ps small hd m vs t2
+  | Fbinop b f1 f2 =>
+    check_decrease_pred fs ps small hd m vs f1 &&
+    check_decrease_pred fs ps small hd m vs f2
+  | Flet t1 v f =>
+    check_decrease_fun fs ps small hd m vs t1 &&
+    check_decrease_pred fs ps (remove vsymbol_eq_dec v small) (upd_option hd v) m vs f
+  | Fif f1 f2 f3 =>
+    check_decrease_pred fs ps small hd m vs f1 &&
+    check_decrease_pred fs ps small hd m vs f2 &&
+    check_decrease_pred fs ps small hd m vs f3
+  | _ => true
+  end.
+
+Lemma funsym_in_tmP: forall fs (t: term),
+  reflect (forall (f: fn), In f fs -> negb (funsym_in_tm (fn_sym f) t))
+    (all (fun f => negb (funsym_in_tm (fn_sym f) t)) fs).
+Proof.
+  move=> fs t.
+  eapply equivP.
+  2: apply Forall_forall.
+  apply forallb_ForallP.
+  move=> x Hinx.
+  apply idP.
+Qed.
+
+Lemma predsym_in_termP: forall ps (t: term),
+  reflect (forall p, In p ps -> negb (predsym_in_term (pn_sym p) t))
+    (all (fun p => negb (predsym_in_term (pn_sym p) t)) ps).
+Proof.
+  move=> ps t.
+  eapply equivP.
+  2: apply Forall_forall.
+  apply forallb_ForallP.
+  move=> x Hinx.
+  apply idP.
+Qed.
+
+Definition fn_eqMixin := EqMixin fn_eqb_spec.
+Canonical fn_eqType := EqType fn fn_eqMixin.
+Definition pn_eqMixin := EqMixin pn_eqb_spec.
+Canonical pn_eqType := EqType pn pn_eqMixin.
+
+(*TODO: 2 others*)
+
+(*Handle case at beginning of most*)
+Ltac not_in_tm_case fs ps t :=
+  case: (all (fun (f: fn) => ~~ (funsym_in_tm (fn_sym f) t)) fs &&
+    all (fun (p: pn) => ~~ (predsym_in_term (pn_sym p) t)) ps)
+    /(andPP (funsym_in_tmP fs t) (predsym_in_termP ps t))=>/=;
+  [move=> [Hnotf Hnotp]; apply ReflectT; by apply Dec_notin_t |].
+
+(*Handle trivial cases for false*)
+Ltac false_triv_case Hnot :=
+  let C := fresh "C" in 
+  apply ReflectF; intro C; inversion C; subst; try by apply Hnot.
+
+Lemma check_decrease_spec fs ps m vs (t: term) (f: formula):
+  NoDup (map fn_sym fs) ->
+  NoDup (map pn_sym ps) ->
+  (forall small hd,
+    reflect (decrease_fun fs ps small hd m vs t)
+      (check_decrease_fun fs ps small hd m vs t)) *
+    (forall small hd,
+      reflect (decrease_pred fs ps small hd m vs f)
+        (check_decrease_pred fs ps small hd m vs f)).
+Proof.
+  move=> Hnodupf Hnodup.
+  move: t f; apply term_formula_rect =>//=;
+  try rewrite orbT.
+  - move=> c small hh.
+    apply ReflectT. apply Dec_const.
+  - move=> v small hd.
+    apply ReflectT. apply Dec_var.
+  - (*Function case - hard one*)
+    move=> f1 tys tms IHall small hd.
+    (*First, handle case where fun/predsyms do not occur*)
+    not_in_tm_case fs ps (Tfun f1 tys tms).
+    (*Now, the main case*)
+    move=> Hnotfp. (*Don't need fun/predsym info anymore*)
+    rewrite -has_find.
+    case: (has (fun f' : fn => fn_sym f' == f1) fs) /hasP => Hhas; last first.
+    {
+      (*First, do non-recursive (in constructed function) case*)
+      have Hnotin: ~ In f1 (List.map fn_sym fs). {
+        rewrite in_map_iff => [[x [Hf1 Hinx]]]; subst.
+        apply Hhas. exists x. by apply/inP. by [].
+      }
+      have Hall: (forall x, x \in tms ->
+        reflect (decrease_fun fs ps small hd m vs x)
+          (check_decrease_fun fs ps small hd m vs x)).
+      { 
+        move {Hnotfp}.
+        move: IHall.
+        elim: tms =>[//= | h t /= IH Hall x].
+        rewrite in_cons.
+        case: (x == h) /eqP => [Hxh _ | Hneq/= Hint]; subst.
+        - apply (ForallT_hd _ _ _ Hall).
+        - apply IH=>//. apply (ForallT_tl _ _ _ Hall).
+      }
+      case: (all [eta check_decrease_fun fs ps small hd m vs] tms)
+        /(all_Forall _ _ _ Hall) => Hall2.
+      - apply ReflectT. apply Dec_fun_notin=>//.
+        by rewrite -Forall_forall.
+      - false_triv_case Hnotfp.
+        (*Now, we have ruled out all cases for decrease_fun*)
+        + apply Hnotin. rewrite in_map_iff.
+          by exists f_decl.
+        + apply Hall2. by apply Forall_forall.   
+    }
+    (*Now we handle the recursive case*)
+    move: Hhas => /hasP Hhas.
+    have /eqP Hnth :=nth_find fn_d Hhas.
+    (*Here, need NoDup, so that f_decl actually equals
+      find ...*)
+    have Hntheq: forall f_decl, In f_decl fs ->
+      f1 = fn_sym f_decl ->
+      f_decl = (nth fn_d fs
+      (find (fun f' : fn => fn_sym f' == fn_sym f_decl) fs)).
+    {
+      move=> f_decl Hin Hf1.
+      apply (NoDup_map_in Hnodupf)=>//.
+      + apply /inP. apply mem_nth. rewrite -has_find. apply /hasP.
+        exists f_decl=>//. by apply /inP.
+      + subst. by rewrite Hnth.
+     }
+    have Hinmap: In f1 (List.map fn_sym fs). {
+      rewrite in_map_iff. eexists. split; [apply Hnth |].
+      apply /inP. apply mem_nth. by rewrite -has_find. 
+    }
+    (*We have to case on the term, only 1 case is interesting;
+      there are a lot of trivial ones*)
+    case Hntht: (nth tm_d tms
+    (sn_idx (nth fn_d fs (find (fun f' : fn => fn_sym f' == f1) fs))))
+    => [| v | | | | |];
+    try (apply ReflectF; intros C; inversion C; subst;
+    try (by apply Hnotfp);
+    try (rewrite -(Hntheq f_decl ltac:(assumption) erefl) in
+      Hntht;
+      match goal with
+      | H1: List.nth ?i ?tms ?tm_d = ?x, H2: nth ?tm_d ?tms ?i = ?y |- _ =>
+        rewrite nth_eq in H1; rewrite H1 in H2; try discriminate end);
+    try contradiction
+    ).
+    case: (v \in small) /inP => Hinv/=; last first.
+    {
+      false_triv_case Hnotfp.
+      rewrite nth_eq in H5. 
+      rewrite -(Hntheq f_decl H2 erefl) in Hntht.
+      rewrite H5 in Hntht. by injection Hntht => Hxy; subst.
+    }
+    case: (tys == map vty_var (s_params f1)) /eqP => Htys/=; last
+    by false_triv_case Hnotfp.
+    (*Hmm- this is annoying - do manually first*)
+    case: ((all (fun t : term => all (fun f : fn => ~~ funsym_in_tm (fn_sym f) t) fs) tms &&
+    all (fun t : term => all (fun p : pn => ~~ predsym_in_term (pn_sym p) t) ps) tms))
+    /(andPP allP allP).
+    + (*The case where we actually say true*)
+      move=> [Hall1 Hall2].
+      apply ReflectT.
+      apply Dec_fun_in with(x:=v)(f_decl:=(nth fn_d fs (find (fun x : fn_eqType => fn_sym x == f1) fs))) =>//.
+      * apply /inP. apply mem_nth. by rewrite -has_find.
+      * by rewrite nth_eq.
+      * rewrite Forall_forall. move=> x /inP Hinx.
+        move: Hall1 => /(_ _ Hinx) /allP Hall1 f /inP Hinf.
+        by apply Hall1.
+      * rewrite Forall_forall. move=> x /inP Hinx.
+        move: Hall2 => /(_ _ Hinx) /allP Hall2 f /inP Hinf.
+        by apply Hall2.
+    + (*One final contradiction case*)
+      move=> /(andPP allP allP).
+      rewrite negb_and.
+      case: (all (fun x : term_eqType => all (fun f : fn => ~~ funsym_in_tm (fn_sym f) x) fs) tms)
+      /allP =>//= [Hall1 Hnotall2 | Hnotall _];
+      false_triv_case Hnotfp. 
+      * move: Hnotall2 => /negP C1. apply C1. apply /allP.
+        move=> t Hint. apply /allP.
+        move=> p Hinp. rewrite Forall_forall in H12. by apply H12; apply /inP.
+      * apply Hnotall. move=> t Hint. apply /allP.
+        move=> f Hinf. rewrite Forall_forall in H11. by apply H11; apply /inP.
+  - move=> tm1 v tm2 IH1 IH2 small hd.
+    not_in_tm_case fs ps (Tlet tm1 v tm2).
+    move => Hnotin.
+    case: (IH1 small hd)=> Hdec1/=; last by false_triv_case Hnotin.
+    case: (IH2 (remove vsymbol_eq_dec v small) (upd_option hd v))=> 
+      Hdec2/=; last by false_triv_case Hnotin.
+    apply ReflectT. by apply Dec_tlet.
+  - (*TODO: automate these cases more*)
+    move=> f t1 t2 IH1 IH2 IH3 small hd.
+    not_in_tm_case fs ps (Tif f t1 t2).
+    move=> Hnotin.
+    case: (IH1 small hd)=> Hdec1/=; last by false_triv_case Hnotin.
+    case: (IH2 small hd)=> Hdec2/=; last by false_triv_case Hnotin.
+    case: (IH3 small hd)=> Hdec3/=; last by false_triv_case Hnotin.
+    apply ReflectT. by apply Dec_tif.
+  - (*Match case - other hard one*) 
+    move=> tm v pats IH1 IHall small hd.
+    not_in_tm_case fs ps (Tmatch tm v pats).
+    move=> Hnotin.
+    move: IH1 Hnotin.
+    (*Most of the cases are the same. First, prove a lemma*)
+    have Hall: forall small hd,
+      reflect (forall x, In x pats ->
+        decrease_fun fs ps (small x) (hd x) m vs (snd x))
+        (all (fun x => check_decrease_fun fs ps (small x) (hd x) m vs (snd x)) pats).
+    {
+      move=> s h. eapply equivP. 2: apply Forall_forall.
+      apply forallb_ForallP.
+      move=> x /inP.
+      move: IHall. elim: pats => [// | h' t' /= IH Hall].
+      rewrite in_cons. case: (x == h') /eqP => Hxh /= => [_ | Hint]; subst.
+      - apply (ForallT_hd _ _ _ Hall).
+      - apply IH=>//. apply (ForallT_tl _ _ _ Hall).
+    }
+    case: tm;
+    (*all cases but 1 are identical*)
+    try (intros; case: (IH1 small hd) => Hdec1/=;
+      [| by false_triv_case Hnotin];
+      case: (Hall (fun x =>(remove_all vsymbol_eq_dec (pat_fv x.1) small) )
+        (fun x => (upd_option_iter hd (pat_fv x.1)))) => Hall1;
+      [| by false_triv_case Hnotin];
+      apply ReflectT; apply Dec_tmatch_rec=>//;
+      move=> [var [Hvar _]]; discriminate).
+    (*Now we come to the variable case*)
+    move=> mvar IH1 Hnotin.
+    case: (@orP ((hd == Some mvar)) ((mvar \in small))) => Hmvar; last first.
+    {
+      case: (Hall (fun x =>(remove_all vsymbol_eq_dec (pat_fv x.1) small) )
+        (fun x => (upd_option_iter hd (pat_fv x.1)))) => Hall1;
+        last first.
+        {
+          false_triv_case Hnotin.
+          apply Hmvar. by case: H2 => Hcon; [left; apply /eqP | right; apply /inP].
+        }
+      apply ReflectT. apply Dec_tmatch_rec=>//.
+      - move=> [var [[Heq] Hvar]]; subst.
+        apply Hmvar. by case: Hvar => Hcon; [left; apply /eqP | right; apply /inP].
+      - by apply Dec_notin_t.
+    }
+    case Hadt: (is_vty_adt gamma (snd mvar)) => [[[m' a'] vs'] |].
+    + apply is_vty_adt_some in Hadt.
+
+    
+    
+    destruct_all; subst.
+    Search is_vty_adt.
+    case Hadt:
+      
+      case: Heq => Heq; subst.
+        
+        false_triv_case Hnotin.
+        apply
+    }
+      
+
+
+
+    + intros. case: (IH1 small hd) => Hdec1/=;
+      last by false_triv_case Hnotin.
+      case: (Hall (fun x =>(remove_all vsymbol_eq_dec (pat_fv x.1) small) )
+        (fun x => (upd_option_iter hd (pat_fv x.1)))) => Hall1;
+      last by false_triv_case Hnotin.
+      apply ReflectT. apply Dec_tmatch_rec=>//.
+      move=> [var [Hvar _]]. discriminate.
+    + admit.
+    + intros. case: (IH1 small hd) => Hdec1/=;
+    last by false_triv_case Hnotin.
+    case: (Hall (fun x =>(remove_all vsymbol_eq_dec (pat_fv x.1) small) )
+      (fun x => (upd_option_iter hd (pat_fv x.1)))) => Hall1;
+    last by false_triv_case Hnotin.
+    apply ReflectT. apply Dec_tmatch_rec=>//.
+    move=> [var [Hvar _]]. discriminate.
+    
+    
+    
+    rewrite /=.
+
+
+
+    {
+      apply ReflectF. move=> C. inversion C; subst;
+      by apply Hnotin.
+    }
+    case: 
+    
+    [Hnot1 Hnot2].
+    case: ((
+      all (fun f => ~~ (funsym_in_tm (fn_sym f) (Tlet tm1 v tm2))) fs && 
+      all (fun p => ~~ (predsym_in_term (pn_sym p) (Tlet tm1 v tm2))) ps)). || predsym_in_term (pn_sym p) tm2)) ps))
+  /(andPP (funsym_in_tmP fs (Tlet tm1 v tm2)) (predsym_in_termP ps (Tlet tm1 v tm2)))=>/=.
+  {
+    move=> [Hnotf Hnotp]. apply ReflectT. by apply Dec_notin_t.
+  }
+      
+      
+      apply
+      
+      /nandP [Hnot1 | Hnto2].
+      Search (negb (?x && ?y)).
+      
+      apply nth_In. apply /inP.
+
+    
+    (funsym_in_tmP fs (Tfun f1 tys tms)) (predsym_in_termP ps (Tfun f1 tys tms)))=>/=.
+
+
+    move: _v_ => v.
+
+      Search List.nth nth.
+    2: {}
+    ).
+    try ()).
+
+
+
+    set (f_decl :=(nth fn_d fs (find (fun x : fn_eqType => fn_sym x == f1) fs))).
+    case: 
+    move Hnth
+
+
+
+    Search has nth find.
+    Search size length.
+    rewrite size_length.
+    Search find reflect.
+
+
+    nth_find:
+  forall [T : Type] (x0 : T) [a : pred T] [s : seq T],
+  has a s -> a (nth x0 s (find a s))
+
+
+    case: (all
+    (fun f : fn =>
+     ~~ (funsym_eq_dec (fn_sym f) f1 || existsb (funsym_in_tm (fn_sym f)) tms)) fs) 
+     /(funsym_in_tmP fs (Tfun f1 tys tms))=>/=;
+    case: (all (fun p0 : pn => ~~ existsb (predsym_in_term (pn_sym p0)) tms) ps)
+    /(predsym_in_termP ps (Tfun f1 tys tms))=>/=.
+
+  
+  
+  Print decrease_fun. constructor. auto.
+
+
+
+  (*Pattern match on var - this is how we add new, smaller variables*)
+ 
+  (*Other pattern match is recursive case*)
+  
+(*This is very similar*)
+with decrease_pred (fs: list fn) (ps: list pn) : 
+  list vsymbol -> option vsymbol -> mut_adt -> list vty -> formula -> Prop :=
+  (*Easy cases: true, false*)
+  | Dec_true: forall (small: list vsymbol) (hd: option vsymbol) m vs,
+    decrease_pred fs ps small hd m vs Ftrue
+  | Dec_false: forall (small: list vsymbol) (hd: option vsymbol) m vs,
+    decrease_pred fs ps small hd m vs Ffalse
+  (*Recursive cases: not, quantifier, eq, binop, let, if*)
+  | Dec_fif: forall (small: list vsymbol) (hd: option vsymbol) m vs
+    (f1 f2 f3: formula),
+    decrease_pred fs ps small hd m vs f1 ->
+    decrease_pred fs ps small hd m vs f2 ->
+    decrease_pred fs ps small hd m vs f3 ->
+    decrease_pred fs ps small hd m vs (Fif f1 f1 f2)
+    .
+
+
+End RecFun.
 
 End ContextCheck.
 
